src/tls/HSL.Receive.fsti
@@ -17,7 +17,7 @@ module HSM = Parsers.Handshake
 module HSM12 = Parsers.Handshake12
 module HSM13 = Parsers.Handshake13
 
-#reset-options "--max_fuel 0 --max_ifuel 0 --using_facts_from '* -FStar.Tactics -FStar.Reflection'"
+#reset-options "--max_fuel 0 --max_ifuel 0 --using_facts_from '* -FStar.Tactics -FStar.Reflection -LowParse'"
 
 
 /// HSL main API
@@ -92,50 +92,10 @@ val create (r:Mem.rgn)
 
 
 /// Receive API
-/// Until a full flight is received, we lose "writing" capability -- as per the comment in HandshakeLog
-
-/// ad-hoc flight types
-/// HS would ask HSL to parse specific flight types, depending on where its own state machine is
 
 type b8 = B.buffer uint_8
 
-module EE  = Parsers.Handshake13_m_encrypted_extensions
-module Fin = Parsers.Handshake13_m_finished
-
-noeq
-type flight_ee_fin = {
-  begin_ee  : uint_32;
-  begin_fin : uint_32;
-  ee_msg    : G.erased EE.handshake13_m_encrypted_extensions;
-  fin_msg   : G.erased Fin.handshake13_m_finished
-}
-
-let valid_flight_t 'a =
-  (flt:'a) -> (flight_end:uint_32) -> (b:b8) -> (h:HS.mem) -> Type0
-
-let valid_parsing13
-  (msg:HSM13.handshake13)
-  (from to:uint_32)
-  (buf:b8{from <= to /\ B.len buf == to - from})
-  (h:HS.mem)
-  = let parser = HSM13.handshake13_parser in
-    let slice = { LP.base = buf; LP.len = to - from } in
-    LP.valid parser h slice from /\
-    LP.contents parser h slice from == msg /\
-    LP.content_length parser h slice from == UInt32.v (to - from)
-
-let valid_flight_ee_fin : valid_flight_t flight_ee_fin =
-  fun (flt:flight_ee_fin) (flight_end:uint_32) (b:b8) (h:HS.mem) ->
-
-  flt.begin_ee <= flt.begin_fin /\
-  flt.begin_fin <= flight_end /\
-  flight_end <= B.len b /\
-
-  (let ee_buf = B.gsub b flt.begin_ee (flt.begin_fin - flt.begin_ee) in
-   let fin_buf = B.gsub b flt.begin_fin (flight_end - flt.begin_fin) in
-   
-   valid_parsing13 (HSM13.M_encrypted_extensions (G.reveal flt.ee_msg)) flt.begin_ee flt.begin_fin ee_buf h /\
-   valid_parsing13 (HSM13.M_finished (G.reveal flt.fin_msg)) flt.begin_fin flight_end fin_buf h)
+#push-options "--max_ifuel 2 --initial_ifuel 2 --z3rlimit 20"  //increase ifuel for inverting options and tuples
 
 let range_extension (r0:option range_t) (from to:uint_32) =
     from <= to /\
@@ -159,7 +119,6 @@ let basic_pre_post (st:hsl_state) (b:b8) (from to:uint_32) : HS.mem -> Type0
     (let start, finish = get_range prev_from_to in
      B.as_seq h (B.gsub b start (finish - start)) == parsed_bytes st h)
 
-#push-options "--max_ifuel 2 --initial_ifuel 2 --z3rlimit 20"
 let update_window (r0:option range_t)
                   (from:uint_32)
                   (to:uint_32{range_extension r0 from to})
@@ -167,6 +126,9 @@ let update_window (r0:option range_t)
   = match r0 with
     | None -> Some (from, to)
     | Some (from_0, _) -> Some (from_0, to)
+
+let valid_flight_t 'a =
+  (flt:'a) -> (flight_begin:uint_32) -> (flight_end:uint_32) -> (b:b8) -> (h:HS.mem) -> Type0
 
 unfold private
 let receive_post 
@@ -189,15 +151,271 @@ let receive_post
        parsed_bytes st h1 == B.as_seq h0 (B.gsub b start (finish - start)) /\
        index_from_to st h1 == update_window (index_from_to st h0) from to
      | Correct (Some flt), None ->
-       f flt to b h1 /\  //flight specific postcondition
+       f flt from to b h1 /\  //flight specific postcondition
        //Internal state for partial parse is reset
        //Ready to receive another flight
        parsed_bytes st h1 == Seq.empty
      | _ -> False)
-#pop-options
+#pop-options //remove the increased ifuel
 
-val receive_flight_ee_fin (st:hsl_state) (b:b8) (from to:uint_32)
-  : ST (TLSError.result (option flight_ee_fin))    //end input buffer index for the flight
+
+/// ad-hoc flight types
+/// HS would ask HSL to parse specific flight types, depending on where its own state machine is
+
+/// First 13 flights
+
+/// Common function for buffer being a valid 13 message msg
+
+let valid_parsing13
+  (msg:HSM13.handshake13)
+  (buf:b8)
+  (h:HS.mem)
+  = let parser = HSM13.handshake13_parser in
+    let slice = { LP.base = buf; LP.len = B.len buf } in
+    LP.valid parser h slice 0ul /\
+    LP.contents parser h slice 0ul == msg /\
+    LP.content_length parser h slice 0ul == B.length buf
+
+
+(****** Flight [ EncryptedExtensions; Certificate13; CertificateVerify; Finished ] ******)
+
+module EE  = Parsers.Handshake13_m_encrypted_extensions
+module C13 = Parsers.Handshake13_m_certificate
+module CV13 = Parsers.Handshake13_m_certificate_verify
+module Fin13 = Parsers.Handshake13_m_finished
+
+noeq
+type flight13_ee_c_cv_fin = {
+  begin_c   : uint_32;
+  begin_cv  : uint_32;
+  begin_fin : uint_32;
+
+  ee_msg  : G.erased EE.handshake13_m_encrypted_extensions;
+  c_msg   : G.erased C13.handshake13_m_certificate;
+  cv_msg  : G.erased CV13.handshake13_m_certificate_verify;
+  fin_msg : G.erased Fin13.handshake13_m_finished
+}
+
+
+let valid_flight13_ee_c_cv_fin
+  : valid_flight_t flight13_ee_c_cv_fin
+  = fun (flt:flight13_ee_c_cv_fin) (flight_begin:uint_32) (flight_end:uint_32) (b:b8) (h:HS.mem) ->
+
+    flight_begin <= flt.begin_c /\
+    flt.begin_c <= flt.begin_cv /\
+    flt.begin_cv <= flt.begin_fin /\
+    flt.begin_fin <= flight_end /\
+    flight_end <= B.len b /\
+
+    (let ee_buf = B.gsub b flight_begin (flt.begin_c - flight_begin) in
+     let c_buf = B.gsub b flt.begin_c (flt.begin_cv - flt.begin_c) in
+     let cv_buf = B.gsub b flt.begin_cv (flt.begin_fin - flt.begin_cv) in
+     let fin_buf = B.gsub b flt.begin_fin (flight_end - flt.begin_fin) in
+
+     valid_parsing13 (HSM13.M_encrypted_extensions (G.reveal flt.ee_msg)) ee_buf h /\
+     valid_parsing13 (HSM13.M_certificate (G.reveal flt.c_msg)) c_buf h /\
+     valid_parsing13 (HSM13.M_certificate_verify (G.reveal flt.cv_msg)) cv_buf h /\
+     valid_parsing13 (HSM13.M_finished (G.reveal flt.fin_msg)) fin_buf h)
+
+
+val receive_flight13_ee_c_cv_fin
+  (st:hsl_state) (b:b8) (from to:uint_32)
+  : ST (TLSError.result (option flight13_ee_c_cv_fin))
+       (requires basic_pre_post st b from to)
+       (ensures  receive_post st b from to valid_flight13_ee_c_cv_fin)
+
+
+(****** Flight [EncryptedExtensions; Certificaterequest13; Certificate13; CertificateVerify; Finished ] ******)
+
+module CR13 = Parsers.Handshake13_m_certificate_request
+
+noeq
+type flight13_ee_cr_c_cv_fin = {
+  begin_cr  : uint_32;
+  begin_c   : uint_32;
+  begin_cv  : uint_32;
+  begin_fin : uint_32;
+
+  ee_msg  : G.erased EE.handshake13_m_encrypted_extensions;
+  cr_msg  : G.erased CR13.handshake13_m_certificate_request;
+  c_msg   : G.erased C13.handshake13_m_certificate;
+  cv_msg  : G.erased CV13.handshake13_m_certificate_verify;
+  fin_msg : G.erased Fin13.handshake13_m_finished
+}
+
+
+let valid_flight13_ee_cr_c_cv_fin
+  : valid_flight_t flight13_ee_cr_c_cv_fin
+  = fun (flt:flight13_ee_cr_c_cv_fin) (flight_begin:uint_32) (flight_end:uint_32) (b:b8) (h:HS.mem) ->
+
+    flight_begin <= flt.begin_cr /\
+    flt.begin_cr <= flt.begin_c /\
+    flt.begin_c <= flt.begin_cv /\
+    flt.begin_cv <= flt.begin_fin /\
+    flt.begin_fin <= flight_end /\
+    flight_end <= B.len b /\
+
+    (let ee_buf = B.gsub b flight_begin (flt.begin_cr - flight_begin) in
+     let cr_buf = B.gsub b flt.begin_cr (flt.begin_c - flt.begin_cr) in 
+     let c_buf = B.gsub b flt.begin_c (flt.begin_cv - flt.begin_c) in
+     let cv_buf = B.gsub b flt.begin_cv (flt.begin_fin - flt.begin_cv) in
+     let fin_buf = B.gsub b flt.begin_fin (flight_end - flt.begin_fin) in
+
+     valid_parsing13 (HSM13.M_encrypted_extensions (G.reveal flt.ee_msg)) ee_buf h /\
+     valid_parsing13 (HSM13.M_certificate_request (G.reveal flt.cr_msg)) cr_buf h /\
+     valid_parsing13 (HSM13.M_certificate (G.reveal flt.c_msg)) c_buf h /\
+     valid_parsing13 (HSM13.M_certificate_verify (G.reveal flt.cv_msg)) cv_buf h /\
+     valid_parsing13 (HSM13.M_finished (G.reveal flt.fin_msg)) fin_buf h)
+
+
+val receive_flight13_ee_cr_c_cv_fin
+  (st:hsl_state) (b:b8) (from to:uint_32)
+  : ST (TLSError.result (option flight13_ee_cr_c_cv_fin))
+       (requires basic_pre_post st b from to)
+       (ensures  receive_post st b from to valid_flight13_ee_cr_c_cv_fin)
+
+
+(****** Flight [EncryptedExtensions; Finished] ******)
+
+noeq
+type flight13_ee_fin = {
+  begin_fin : uint_32;
+
+  ee_msg    : G.erased EE.handshake13_m_encrypted_extensions;
+  fin_msg   : G.erased Fin13.handshake13_m_finished
+}
+
+let valid_flight13_ee_fin : valid_flight_t flight13_ee_fin =
+  fun (flt:flight13_ee_fin) (flight_begin:uint_32) (flight_end:uint_32) (b:b8) (h:HS.mem) ->
+
+  flight_begin <= flt.begin_fin /\
+  flt.begin_fin <= flight_end /\
+  flight_end <= B.len b /\
+
+  (let ee_buf = B.gsub b flight_begin (flt.begin_fin - flight_begin) in
+   let fin_buf = B.gsub b flt.begin_fin (flight_end - flt.begin_fin) in
+   
+   valid_parsing13 (HSM13.M_encrypted_extensions (G.reveal flt.ee_msg)) ee_buf h /\
+   valid_parsing13 (HSM13.M_finished (G.reveal flt.fin_msg)) fin_buf h)
+
+val receive_flight13_ee_fin (st:hsl_state) (b:b8) (from to:uint_32)
+  : ST (TLSError.result (option flight13_ee_fin))
        (requires basic_pre_post st b  from to)
-       (ensures  receive_post st b from to valid_flight_ee_fin)
+       (ensures  receive_post st b from to valid_flight13_ee_fin)
 
+
+(****** Flight [ Finished ] ******)
+
+noeq
+type flight13_fin = {
+  fin_msg : G.erased Fin13.handshake13_m_finished
+}
+
+
+let valid_flight13_fin : valid_flight_t flight13_fin =
+  fun (flt:flight13_fin) (flight_begin:uint_32) (flight_end:uint_32) (b:b8) (h:HS.mem) ->
+
+  flight_begin <= flight_end /\
+  flight_end <= B.len b /\
+
+  (let fin_buf = B.gsub b flight_begin (flight_end - flight_begin) in
+   
+   valid_parsing13 (HSM13.M_finished (G.reveal flt.fin_msg)) fin_buf h)
+
+val receive_flight13_fin (st:hsl_state) (b:b8) (from to:uint_32)
+  : ST (TLSError.result (option flight13_fin))
+       (requires basic_pre_post st b  from to)
+       (ensures  receive_post st b from to valid_flight13_fin)
+
+
+(****** Flight [ Certificate13; CertificateVerify; Finished ] ******)
+
+noeq
+type flight13_c_cv_fin = {
+  begin_cv  : uint_32;
+  begin_fin : uint_32;
+
+  c_msg   : G.erased C13.handshake13_m_certificate;
+  cv_msg  : G.erased CV13.handshake13_m_certificate_verify;
+  fin_msg : G.erased Fin13.handshake13_m_finished
+}
+
+
+let valid_flight13_c_cv_fin
+  : valid_flight_t flight13_c_cv_fin
+  = fun (flt:flight13_c_cv_fin) (flight_begin:uint_32) (flight_end:uint_32) (b:b8) (h:HS.mem) ->
+
+    flight_begin <= flt.begin_cv /\
+    flt.begin_cv <= flt.begin_fin /\
+    flt.begin_fin <= flight_end /\
+    flight_end <= B.len b /\
+
+    (let c_buf = B.gsub b flight_begin (flt.begin_cv - flight_begin) in
+     let cv_buf = B.gsub b flt.begin_cv (flt.begin_fin - flt.begin_cv) in
+     let fin_buf = B.gsub b flt.begin_fin (flight_end - flt.begin_fin) in
+
+     valid_parsing13 (HSM13.M_certificate (G.reveal flt.c_msg)) c_buf h /\
+     valid_parsing13 (HSM13.M_certificate_verify (G.reveal flt.cv_msg)) cv_buf h /\
+     valid_parsing13 (HSM13.M_finished (G.reveal flt.fin_msg)) fin_buf h)
+
+
+val receive_flight13_c_cv_fin
+  (st:hsl_state) (b:b8) (from to:uint_32)
+  : ST (TLSError.result (option flight13_c_cv_fin))
+       (requires basic_pre_post st b from to)
+       (ensures  receive_post st b from to valid_flight13_c_cv_fin)
+
+
+(****** Flight [ EndOfEarlyData ] ******)
+
+module EoED13 = Parsers.Handshake13_m_end_of_early_data
+
+noeq
+type flight13_eoed = {
+  eoed_msg : G.erased (EoED13.handshake13_m_end_of_early_data)
+}
+
+
+let valid_flight13_eoed : valid_flight_t flight13_eoed =
+  fun (flt:flight13_eoed) (flight_begin:uint_32) (flight_end:uint_32) (b:b8) (h:HS.mem) ->
+
+  flight_begin <= flight_end /\
+  flight_end <= B.len b /\
+
+  (let eoed_buf = B.gsub b flight_begin (flight_end - flight_begin) in
+   
+   valid_parsing13 (HSM13.M_end_of_early_data (G.reveal flt.eoed_msg)) eoed_buf h)
+
+val receive_flight13_eoed (st:hsl_state) (b:b8) (from to:uint_32)
+  : ST (TLSError.result (option flight13_eoed))
+       (requires basic_pre_post st b  from to)
+       (ensures  receive_post st b from to valid_flight13_eoed)
+
+
+(****** Flight [ NewSessionTicket13 ] ******)
+
+module NST13 = Parsers.Handshake13_m_new_session_ticket
+
+noeq
+type flight13_nst = {
+  nst_msg : G.erased (NST13.handshake13_m_new_session_ticket)
+}
+
+
+let valid_flight13_nst : valid_flight_t flight13_nst =
+  fun (flt:flight13_nst) (flight_begin:uint_32) (flight_end:uint_32) (b:b8) (h:HS.mem) ->
+
+  flight_begin <= flight_end /\
+  flight_end <= B.len b /\
+
+  (let nst_buf = B.gsub b flight_begin (flight_end - flight_begin) in
+   
+   valid_parsing13 (HSM13.M_new_session_ticket (G.reveal flt.nst_msg)) nst_buf h)
+
+val receive_flight13_nst (st:hsl_state) (b:b8) (from to:uint_32)
+  : ST (TLSError.result (option flight13_nst))
+       (requires basic_pre_post st b  from to)
+       (ensures  receive_post st b from to valid_flight13_nst)
+
+
+/// TODO: 12 flights
